theories/logic/spec_rules.v
@@ -160,11 +160,11 @@ Section rules.
     iMod (own_update with "Hown") as "[Hown Hl]".
     { eapply auth_update_alloc, prod_local_update_2,
         (alloc_singleton_local_update _ l (1%Qp,to_agree (Some v : leibnizO _))); last done.
-      by apply lookup_to_gen_heap_None. }
+      by apply lookup_to_heap_None. }
     rewrite heapS_mapsto_eq /heapS_mapsto_def /=.
     iExists l. iFrame "Hj Hl". iApply "Hclose". iNext.
     iExists (<[j:=fill K (# l)]> tp), (state_upd_heap <[l:=Some v]> σ).
-    rewrite to_gen_heap_insert to_tpool_insert'; last eauto. iFrame. iPureIntro.
+    rewrite to_heap_insert to_tpool_insert'; last eauto. iFrame. iPureIntro.
     eapply rtc_r, step_insert_no_fork; eauto.
     rewrite -state_init_heap_singleton. eapply AllocNS; first by lia.
     intros. assert (i = 0) as -> by lia. by rewrite loc_add_0.
@@ -183,7 +183,7 @@ Section rules.
     iDestruct (own_valid_2 with "Hown Hj")
       as %[[?%tpool_singleton_included' _]%prod_included ?]%auth_both_valid_discrete.
     iDestruct (own_valid_2 with "Hown Hl")
-      as %[[? ?%gen_heap_singleton_included]%prod_included ?]%auth_both_valid_discrete.
+      as %[[? ?%heap_singleton_included]%prod_included ?]%auth_both_valid_discrete.
     iMod (own_update_2 with "Hown Hj") as "[Hown Hj]".
     { by eapply auth_update, prod_local_update_1, singleton_local_update,
         (exclusive_local_update _ (Excl (fill K (of_val v)))). }
@@ -207,20 +207,20 @@ Section rules.
     iDestruct (own_valid_2 with "Hown Hj")
       as %[[?%tpool_singleton_included' _]%prod_included _]%auth_both_valid_discrete.
     iDestruct (own_valid_2 with "Hown Hl")
-      as %[[_ Hl%gen_heap_singleton_included]%prod_included _]%auth_both_valid_discrete.
+      as %[[_ Hl%heap_singleton_included]%prod_included _]%auth_both_valid_discrete.
     iMod (own_update_2 with "Hown Hj") as "[Hown Hj]".
     { by eapply auth_update, prod_local_update_1, singleton_local_update,
         (exclusive_local_update _ (Excl (fill K #()))). }
     iMod (own_update_2 with "Hown Hl") as "[Hown Hl]".
     { eapply auth_update, prod_local_update_2.
       apply: singleton_local_update.
-      { by rewrite /to_gen_heap lookup_fmap Hl. }
+      { by rewrite /to_heap lookup_fmap Hl. }
       apply: (exclusive_local_update _
         (1%Qp, to_agree (Some v : leibnizO (option val)))).
       apply: pair_exclusive_l. done. }
     iFrame "Hj Hl". iApply "Hclose". iNext.
     iExists (<[j:=fill K #()]> tp), (state_upd_heap <[l:=Some v]> σ).
-    rewrite to_gen_heap_insert to_tpool_insert'; last eauto. iFrame. iPureIntro.
+    rewrite to_heap_insert to_tpool_insert'; last eauto. iFrame. iPureIntro.
     eapply rtc_r, step_insert_no_fork; eauto. econstructor; eauto.
   Qed.
 
@@ -241,7 +241,7 @@ Section rules.
     iDestruct (own_valid_2 with "Hown Hj")
       as %[[?%tpool_singleton_included' _]%prod_included ?]%auth_both_valid_discrete.
     iDestruct (own_valid_2 with "Hown Hl")
-      as %[[_ ?%gen_heap_singleton_included]%prod_included _]%auth_both_valid_discrete.
+      as %[[_ ?%heap_singleton_included]%prod_included _]%auth_both_valid_discrete.
     iMod (own_update_2 with "Hown Hj") as "[Hown Hj]".
     { by eapply auth_update, prod_local_update_1, singleton_local_update,
         (exclusive_local_update _ (Excl (fill K (_, #false)%V))). }
@@ -268,20 +268,20 @@ Section rules.
     iDestruct (own_valid_2 with "Hown Hj")
       as %[[?%tpool_singleton_included' _]%prod_included _]%auth_both_valid_discrete.
     iDestruct (own_valid_2 with "Hown Hl")
-      as %[[_ Hl%gen_heap_singleton_included]%prod_included _]%auth_both_valid_discrete.
+      as %[[_ Hl%heap_singleton_included]%prod_included _]%auth_both_valid_discrete.
     iMod (own_update_2 with "Hown Hj") as "[Hown Hj]".
     { by eapply auth_update, prod_local_update_1, singleton_local_update,
         (exclusive_local_update _ (Excl (fill K (_, #true)%V))). }
     iMod (own_update_2 with "Hown Hl") as "[Hown Hl]".
     { eapply auth_update, prod_local_update_2.
       apply: singleton_local_update.
-      { by rewrite /to_gen_heap lookup_fmap Hl. }
+      { by rewrite /to_heap lookup_fmap Hl. }
       apply: (exclusive_local_update _
         (1%Qp, to_agree (Some v2 : leibnizO (option val)))).
       apply: pair_exclusive_l. done. }
     iFrame "Hj Hl". iApply "Hclose". iNext.
     iExists (<[j:=fill K (_, #true)%V]> tp), (state_upd_heap <[l:=Some v2]> σ).
-    rewrite to_gen_heap_insert to_tpool_insert'; last eauto. iFrame. iPureIntro.
+    rewrite to_heap_insert to_tpool_insert'; last eauto. iFrame. iPureIntro.
     eapply rtc_r, step_insert_no_fork; eauto. econstructor; eauto.
     rewrite bool_decide_true //.
   Qed.
@@ -299,20 +299,20 @@ Section rules.
     iDestruct (own_valid_2 with "Hown Hj")
       as %[[?%tpool_singleton_included' _]%prod_included _]%auth_both_valid_discrete.
     iDestruct (own_valid_2 with "Hown Hl")
-      as %[[_ Hl%gen_heap_singleton_included]%prod_included _]%auth_both_valid_discrete.
+      as %[[_ Hl%heap_singleton_included]%prod_included _]%auth_both_valid_discrete.
     iMod (own_update_2 with "Hown Hj") as "[Hown Hj]".
     { by eapply auth_update, prod_local_update_1, singleton_local_update,
         (exclusive_local_update _ (Excl (fill K (# i1)))). }
     iMod (own_update_2 with "Hown Hl") as "[Hown Hl]".
     { eapply auth_update, prod_local_update_2.
       apply: singleton_local_update.
-      { by rewrite /to_gen_heap lookup_fmap Hl. }
+      { by rewrite /to_heap lookup_fmap Hl. }
       apply: (exclusive_local_update _
         (1%Qp, to_agree (Some #(i1+i2) : leibnizO (option val)))).
       apply: pair_exclusive_l. done. }
     iFrame "Hj Hl". iApply "Hclose". iNext.
     iExists (<[j:=fill K (# i1)]> tp), (state_upd_heap <[l:=Some #(i1+i2)]> σ).
-    rewrite to_gen_heap_insert to_tpool_insert'; last eauto. iFrame. iPureIntro.
+    rewrite to_heap_insert to_tpool_insert'; last eauto. iFrame. iPureIntro.
     eapply rtc_r, step_insert_no_fork; eauto. simpl. econstructor; eauto.
   Qed.
 
